

① LP ② NLP. ③ IP. ④ GP/BA

Gradient Decent (Min). Gradient Ascent (Max)

= Steepest descent (ascent).

$\max f(x,y) = 2xy + 2y - x^2 - 2y^2$. (A concave by Hessian matrix)

$$\frac{\partial f}{\partial x} = 2y - 2x = 0 \Rightarrow y = x$$

$$\frac{\partial f}{\partial y} = 2x + 2 - 4y = 0, \quad 2x + 2 - 4y = 0, \quad -2x = -2.$$

$x=1, y=1$. (1,1) is global
max.

The idea of gradient ascent:

$$\vec{x}_{t+1} = \vec{x}_t + \alpha \nabla f(\vec{x}_t) \quad , \quad t=0, 1, 2, \dots$$

$$\vec{x}_1 = \vec{x}_0 + \alpha \cdot \nabla f(\vec{x}_0) \quad \text{first point is added by initial } \alpha$$

directional small
step.

↙

direction is the ∇ .
step size = α .

initial point can be achieved arbitrarily :

$$\text{let } \vec{x}_0 = (2, 0) ,$$

$$\nabla f = \begin{bmatrix} 2y - 2x \\ 2x + \text{---} - 4y \end{bmatrix} .$$

$$\bar{x}_1 = \begin{pmatrix} 0 \\ 0 \end{pmatrix} + \alpha \cdot \begin{pmatrix} 2 \cdot 0 - 2 \cdot 0 \\ 2 \cdot 0 + 2 - 4 \cdot 0 \end{pmatrix}$$

$$\bar{x}_1 = \begin{pmatrix} 0 \\ 0 \end{pmatrix} + \alpha \cdot \begin{pmatrix} 0 \\ 2 \end{pmatrix}.$$

$\bar{x}_1 = \begin{pmatrix} 0 \\ 2\alpha \end{pmatrix}$ we have to determine α .

we have to put $\begin{cases} x=0 \\ y=2\alpha \end{cases}$ in to original function,

$$f(x, y) = 2 \cdot 0 \cdot 2\alpha + 2 \cdot 2\alpha - 0 - 2 \cdot 4\alpha^2$$

$$= 0 + 4\alpha - 8\alpha^2.$$

$$= 4\alpha - 8\alpha^2$$

we have to maximize this (f) .

$$2xy + 2y - x^2 - 2y^2.$$

$$\frac{\partial f}{\partial \alpha} = 4 - 16\alpha = 0, \quad \alpha = \frac{1}{4}, \quad \text{i.e. } \alpha = \frac{1}{4} \text{ maximizes the } \alpha.$$

$$\text{i.e. } \bar{x}_1 = \begin{pmatrix} 0 \\ \frac{1}{2} \end{pmatrix} = \begin{pmatrix} 0 \\ 0.5 \end{pmatrix}$$

$$\bar{x}_{t+1} = \bar{x}_t + \alpha \cdot \nabla f(\bar{x}_t)$$

$$\bar{x}_2 = \bar{x}_1 + \alpha \cdot \nabla f(\bar{x}_1)$$

$$\nabla f = \begin{bmatrix} 2y - 2x \\ 2x + 2 - 4y \end{bmatrix}$$

$$\nabla f \begin{pmatrix} 0 \\ 0.5 \end{pmatrix} = \begin{pmatrix} 1 - 0 \\ 0 + 2 - 2 \end{pmatrix} = \begin{pmatrix} 1 \\ 0 \end{pmatrix}$$

$$\bar{x}_2 = \begin{pmatrix} 0 \\ 0.5 \end{pmatrix} + \alpha \cdot \begin{pmatrix} 1 \\ 0 \end{pmatrix}$$

$$\bar{x}_2 = \begin{pmatrix} \alpha \\ 0.5 \end{pmatrix}$$

$$2xy + 2y - x^2 - 2y^2$$

$$f(\bar{x}_2) = 2\alpha \cdot \frac{1}{2} + 2 \cdot \frac{1}{2} - \alpha^2 - 2 \cdot \frac{1}{4}$$

$$= \alpha + 1 - \alpha^2 - \frac{1}{2}$$

$$= -\alpha^2 + \alpha + \frac{1}{2}$$

$$\frac{df}{d\alpha} = -2\alpha + 1 = 0 \quad -2\alpha = -1$$

$$\alpha = \frac{1}{2} = 0.5 \quad \therefore \bar{x}_2 = \begin{pmatrix} 0.5 \\ 0.5 \end{pmatrix}$$

$$\bar{x}_3 = \begin{pmatrix} 0.5 \\ 0.5 \end{pmatrix} + \alpha \cdot \begin{pmatrix} 0 \\ 1 \end{pmatrix}$$

$$\bar{x}_3 = \begin{pmatrix} 0.5 \\ 0.5 + \alpha \end{pmatrix}$$

$$\nabla f(\bar{x}_2) = \begin{pmatrix} 2 \times \frac{1}{2} - 2 \times \frac{1}{2} \\ 2 \times \frac{1}{2} + 2 - 4 \times \frac{1}{2} \end{pmatrix} = \begin{pmatrix} 0 \\ 1 \end{pmatrix}$$

$$1 + 2 - 2$$

$$2xy + 2y - x^2 - 2y^2.$$

$$f(\bar{X}_3) = 2 \times 0.5 \times (0.5 + \alpha) + 2(0.5 + \alpha) - \frac{1}{4} - 2 \times (0.5 + \alpha)^2$$

$$= 3(0.5 + \alpha) - \frac{1}{4} - 2 \times (0.5 + \alpha)^2.$$

$$= \frac{6}{4} + 3\alpha - \frac{1}{4} - 2 \times \left(\frac{1}{4} + \alpha + \alpha^2 \right).$$

$$= \frac{5}{4} + 3\alpha - \frac{1}{4} - 2\alpha - 2\alpha^2.$$

$$= -2\alpha^2 + \alpha + \frac{3}{4}.$$

$$\frac{\partial f}{\partial \alpha} = -4\alpha + 1.$$

$$-4\alpha + 1 = 0 \Rightarrow \alpha = \frac{1}{4}.$$

$$i) \bar{x}_3 = \begin{pmatrix} \frac{1}{2} \\ \frac{3}{4} \end{pmatrix}, \dots$$

$$\nabla f = \begin{bmatrix} 2y - 2x \\ 2x + 2 - 4y \end{bmatrix}.$$

$$\bar{x}_4 = \bar{x}_3 + \alpha \cdot \nabla f(\bar{x}_3)$$

$$\nabla f(\bar{x}_3) = \begin{pmatrix} \frac{3}{2} - 1 = \frac{1}{2} \\ 2 \times \frac{1}{2} + 2 - 4 \times \frac{3}{4} \end{pmatrix}$$

$$\bar{x}_4 = \begin{pmatrix} \frac{1}{2} \\ \frac{3}{4} \end{pmatrix} + \alpha \cdot \begin{pmatrix} \frac{1}{2} \\ 0 \end{pmatrix}$$

$$= \begin{pmatrix} \frac{1}{2} \\ 0 \end{pmatrix}.$$

$$\bar{x}_4 = \begin{pmatrix} \frac{1}{2} + \alpha \cdot \frac{1}{2} \\ \frac{3}{4} \end{pmatrix} = \begin{pmatrix} \frac{1}{2}(1 + \alpha) \\ \frac{3}{4} \end{pmatrix}$$

$$2xy + 2y - x^2 - 2y^2.$$

$$f = 2 \times \frac{1}{2}(1 + \alpha) \cdot \frac{3}{4} + 2 \times \frac{3}{4} - \frac{1}{4}(1 + \alpha)^2 - 2 \times \frac{9}{16}$$

$$= \frac{3}{4}(1+\alpha) + \frac{3}{2} - \frac{1}{4}(1+2\alpha+\alpha^2) - \frac{9}{8}$$

$$\frac{\partial f}{\partial \alpha} = \frac{3}{4} - \frac{1}{4}[2+2\alpha] = 0$$

$$3 = 1 + 2\alpha$$

$$1 = 2\alpha \Rightarrow \alpha = \frac{1}{2}$$

$$\therefore \bar{x}_4 = \begin{pmatrix} \frac{1}{2}(1 + \frac{1}{2}) \\ \frac{3}{4} \end{pmatrix} = \begin{pmatrix} \frac{3}{4} \\ \frac{3}{4} \end{pmatrix}$$

$$2y - 2x = 0 \quad -1$$

$$2x + 2 - 4y = \frac{3}{2} + 2 - 4 \cdot \frac{3}{4}$$

$$= \frac{2}{2} - \frac{2}{2} = \frac{1}{2}$$

$$\therefore \bar{x}_5 = \begin{pmatrix} \frac{3}{4} \\ \frac{3}{4} \end{pmatrix} + \alpha \cdot \begin{pmatrix} 0 \\ \frac{1}{2} \end{pmatrix}$$

$$\bar{x}_5 = \begin{pmatrix} \frac{3}{4} \\ \frac{3}{4} + \frac{1}{2}\alpha \end{pmatrix}.$$

$$2xy + 2y - x^2 - 2y^2.$$

$$f = 2 \times \frac{3}{4} \times (\frac{3}{4} + \frac{1}{2}\alpha) + 2 \times (\frac{3}{4} + \frac{1}{2}\alpha) - \frac{9}{16} - 2 \times (\frac{3}{4} + \frac{1}{2}\alpha)^2$$

$$= 2 \times \frac{3}{4} \times \frac{3}{4} + 2 \times \frac{3}{4} \times \frac{1}{2}\alpha + 2 \times \frac{3}{4} + \alpha - \frac{9}{16} - 2 \times$$

$$(\frac{9}{16} + \frac{3}{4}\alpha + \frac{1}{4}\alpha^2).$$

$$= \frac{3}{4}\alpha + \alpha - 2 \times \frac{3}{4}\alpha - 2 \times \frac{1}{4}\alpha^2 + \dots$$

$$= \frac{1}{4}\alpha - \frac{1}{2}\alpha^2 + \dots$$

$$\frac{\partial f}{\partial \alpha} = -\frac{1}{2} \times 2\alpha + \frac{1}{4}$$

$$\alpha = \frac{1}{4}.$$

$$= -\alpha + \frac{1}{4}$$

$$\bar{X}_5 = \begin{pmatrix} \frac{3}{4} \\ \frac{3}{4} + \frac{1}{2} \cdot \frac{1}{4} \end{pmatrix} = \begin{pmatrix} \frac{3}{4} \\ \frac{7}{8} \end{pmatrix}$$

$$2y - 2x = 2x \cdot \frac{7}{8} - 2x \cdot \frac{3}{4} \\ = \frac{1}{4}$$

$$\bar{X}_6 = \begin{pmatrix} \frac{3}{4} \\ \frac{7}{8} \end{pmatrix} + \alpha \cdot \begin{pmatrix} \frac{1}{4} \\ 0 \end{pmatrix}$$

$$2x + 2 - 4y = 2x \cdot \frac{3}{4} + 2 - 4x \cdot \frac{7}{8}$$

$$= \frac{3+4}{2} - \frac{7}{2} = 0$$

$$\bar{X}_6 = \begin{pmatrix} \frac{3}{4} + \frac{1}{4}\alpha \\ \frac{7}{8} \end{pmatrix} \quad \frac{1}{4}(3+\alpha)$$

$$9 + 6\alpha + \alpha^2$$

$$f(\alpha) = 2x \cdot \frac{1}{4}(3+\alpha) \cdot \frac{7}{8} + 2x \cdot \frac{7}{8} - \frac{1}{16}(3+\alpha)^2 - 2x \cdot \frac{56}{64}$$

$$\frac{7}{16}\alpha - \frac{1}{16} \times 6\alpha - \frac{1}{16} \cdot \alpha^2$$

$$\frac{\partial f}{\partial \alpha} = -\frac{1}{8}\alpha + \frac{1}{16} = 0 \Rightarrow \frac{1}{8}\alpha = \frac{1}{16}$$

$$2\alpha = 1, \quad \alpha = \frac{1}{2}$$

$$\hat{x}_0 = \begin{pmatrix} \frac{3}{4} + \frac{1}{4} \times \frac{1}{2} \\ \frac{7}{8} \end{pmatrix} = \begin{pmatrix} \frac{7}{8} \\ \frac{7}{8} \end{pmatrix}$$

..... skipped. final result = (1, 1)